TM/LM/Alphabets.v
@@ -1,0 +1,75 @@
+Require Import TM.Prelim.
+Require Import TM.Code.Code.
+Require Import Semantics.
+
+(** * Alphabets *)
+
+(* See [TokTM] *)
+
+Inductive ATok : Type := retAT | lamAT | appAT.
+
+Coercion ATok2Tok (a : ATok) : Tok :=
+  match a with
+  | retAT => retT
+  | lamAT => lamT
+  | appAT => appT
+  end.
+
+
+Instance ATok_eq_dec : eq_dec ATok.
+Proof. intros x y; hnf. decide equality. Defined.
+
+Instance ATok_finType : finTypeC (EqType ATok).
+Proof. split with (enum := [retAT; lamAT; appAT]). intros [ | | ]; cbn; reflexivity. Defined.
+
+Instance ATok_inhab : inhabitedC ATok := ltac:(repeat constructor).
+
+Instance Encode_ATok : codable ATok ATok := Encode_Finite (FinType(EqType ATok)).
+
+
+Coercion Tok_to_sum (t : Tok) : (nat + ATok) :=
+  match t with
+  | varT x => inl x
+  | appT => inr appAT
+  | lamT => inr lamAT
+  | retT => inr retAT
+  end.
+
+Definition sigTok := sigSum sigNat ATok.
+Definition sigTok_fin := FinType (EqType sigTok).
+
+Instance Encode_Tok : codable sigTok Tok :=
+  {|
+    encode x := encode (Tok_to_sum x)
+  |}.
+
+Definition Encode_Tok_size (t : Tok) : nat :=
+  size _ (Tok_to_sum t).
+
+Lemma Encode_Tok_hasSize (t : Tok) :
+  size _ t = Encode_Tok_size t.
+Proof. reflexivity. Qed.
+
+
+Definition sigHAd := sigNat.
+Definition sigHAd_fin := FinType(EqType sigHAd).
+
+Definition sigPro := sigList sigTok.
+Instance Encode_Prog : codable sigPro Pro := _.
+Definition sigPro_fin := FinType(EqType sigPro).
+
+Definition sigHClos := sigPair sigHAd sigPro.
+Definition sigHClos_fin := FinType(EqType sigHClos).
+Instance Encode_HClos : codable sigHClos HClos := _.
+
+Definition sigHEnt' := sigPair sigHClos sigHAd.
+Instance Encode_HEnt' : codable (sigHEnt') (HClos*HAd) := _.
+Definition sigHEnt'_fin := FinType(EqType sigHEnt').
+
+Definition sigHEnt := sigOption sigHEnt'.
+Instance Encode_HEnt : codable (sigHEnt) HEnt := _.
+Definition sigHEnt_fin := FinType(EqType sigHEnt).
+
+Definition sigHeap := sigList sigHEnt.
+Instance Encode_Heap : codable (sigHeap) Heap := _.
+Definition sigHeap_fin := FinType(EqType sigHeap).
